Add saved-regs to new Rec call in bignum mini

compiler/backend/proofs/word_bignumProofScript.sml
@@ -2,6 +2,7 @@ open preamble astTheory wordLangTheory wordSemTheory tailrecTheory;
 open mc_multiwordTheory set_sepTheory helperLib word_bignumTheory;
 
 val good_dimindex_def = labPropsTheory.good_dimindex_def;
+val env_to_list_lookup_equiv = wordPropsTheory.env_to_list_lookup_equiv;
 
 val _ = new_theory "word_bignumProof";
 
@@ -59,6 +60,13 @@ val array_write_def = Define `
 val clock_write_def = Define `
   clock_write l s = s with clock := l`;
 
+val copy_vars_def = Define `
+  (copy_vars [] s t = SOME t) /\
+  (copy_vars (n::ns) s t =
+     case FLOOKUP s n of
+     | NONE => NONE
+     | SOME x => copy_vars ns s (reg_write n (SOME x) t))`;
+
 val (eval_rules,eval_ind,raw_eval_cases) = Hol_reln `
   (!r s. Eval r s Skip (INR (s:'a state))) /\
   (!r s. Eval r s Continue (INL s)) /\
@@ -112,10 +120,11 @@ val (eval_rules,eval_ind,raw_eval_cases) = Hol_reln `
      Eval (if rec then SOME p else NONE) (delete_vars vs (dec_clock s1))
        (LoopBody p) (INR s2) /\ s1.clock <> 0 ==>
      Eval r s1 (Loop rec vs p) (INR s2)) /\
-  (!s1 vs p s2.
+  (!s1 save_regs vs p s2 s3.
      Eval (SOME p) (delete_vars vs (dec_clock s1)) (LoopBody p) (INR s2) /\
+     copy_vars save_regs s1.regs s2 = SOME s3 /\
      s1.clock <> 0 ==>
-     Eval (SOME p) s1 (Rec vs) (INR s2)) /\
+     Eval (SOME p) s1 (Rec save_regs vs) (INR s3)) /\
   (!r s1 p s2.
      Eval r s1 p (INR s2) ==>
      Eval r s1 (LoopBody p) (INR s2)) /\
@@ -139,7 +148,7 @@ val eval_cases =
      ``Eval rec s1 (Sub r1 r2 r3 r4 r5) s2``,
      ``Eval rec s1 (Mul r1 r2 r3 r4) s2``,
      ``Eval rec s1 (Div r1 r2 r3 r4 r5) s2``,
-     ``Eval rec s1 (Rec vs) s2``,
+     ``Eval rec s1 (Rec save_regs vs) s2``,
      ``Eval rec s1 (Loop r vs p) s2``,
      ``Eval rec s1 (LoopBody p) s2``] |> LIST_CONJ;
 
@@ -267,6 +276,8 @@ val syntax_ok_aux_def = Define `
   (syntax_ok_aux (Div n1 n2 n3 n4 n5) <=>
      n1 < max_var_name /\ n2 < max_var_name /\
      n3 < max_var_name /\ n4 < max_var_name /\ n5 < max_var_name) /\
+  (syntax_ok_aux (Rec save_regs _) <=>
+     EVERY (\n. n < max_var_name) save_regs /\ ALL_DISTINCT save_regs) /\
   syntax_ok_aux _ = T`;
 
 val syntax_ok_def = Define `
@@ -424,6 +435,125 @@ val b2w_if = prove(
 val b2n_if = prove(
   ``b2n b = if ~b then 0 else 1``,
   Cases_on `b` \\ EVAL_TAC);
+
+val list_update_def = Define `
+  list_update [] ys t = t /\
+  list_update (x::xs) (y::ys) t = insert x y (list_update xs ys t) /\
+  list_update (x::xs) [] t = insert x ARB (list_update xs [] t)`
+
+val evaluate_LoadRegs = prove(
+  ``!save_regs vals t1.
+      state_rel s1 t1 cs2 t0 frame /\
+      EVERY (λn. n < max_var_name) save_regs /\ ALL_DISTINCT save_regs /\
+      EVERY2 (\n v. FLOOKUP s1.regs n = SOME v) save_regs vals ==>
+      evaluate (LoadRegs save_regs p, t1) =
+      evaluate (p, t1 with locals :=
+           list_update (MAP (\n. n+2) save_regs) (MAP Word vals) t1.locals)``,
+  Induct \\ fs [LoadRegs_def,list_update_def]
+  THEN1 (rw [] \\ AP_TERM_TAC \\ fs [wordSemTheory.state_component_equality])
+  \\ rw [] \\ fs [evaluate_def]
+  \\ qpat_assum `state_rel _ _ _ _ _` (mp_tac o REWRITE_RULE [state_rel_def])
+  \\ strip_tac
+  \\ first_x_assum drule \\ strip_tac \\ fs []
+  \\ `state_rel s1 (set_var (h + 2) (Word v) t1) cs2 t0 frame` by
+        fs [state_rel_def,set_var_def]
+  \\ first_x_assum drule
+  \\ disch_then drule
+  \\ fs [] \\ rw [] \\ AP_TERM_TAC \\ fs []
+  \\ fs [set_var_def,list_update_def]
+  \\ rpt (AP_THM_TAC ORELSE AP_TERM_TAC) \\ fs []
+  \\ imp_res_tac LIST_REL_LENGTH \\ pop_assum mp_tac
+  \\ qpat_x_assum `¬MEM h save_regs` mp_tac
+  \\ qpat_x_assum `EVERY _ _` mp_tac
+  \\ qpat_x_assum `_ < _:num` mp_tac
+  \\ rpt (pop_assum kall_tac)
+  \\ qspec_tac (`ys`,`ys`)
+  \\ qspec_tac (`save_regs`,`xs`)
+  \\ Induct \\ Cases_on `ys` \\ fs [list_update_def]
+  \\ simp [Once insert_insert]);
+
+val domain_list_update = prove(
+  ``∀xs ys x t. x ∈ domain (list_update xs ys t) ⇔ MEM x xs ∨ x ∈ domain t``,
+  Induct \\ Cases_on `ys` \\ fs [list_update_def] \\ metis_tac []);
+
+val list_store_def = Define `
+  list_store [] ys s = s /\
+  list_store (x::xs) ys s = (list_store xs (TL ys) s) |+ (Temp (n2w x),HD ys)`
+
+val list_store_FUPDATE = prove(
+  ``!save_regs st ys.
+      ¬MEM h save_regs /\ h < max_var_name /\
+      EVERY (λn. n < max_var_name) save_regs ==>
+      list_store save_regs ys (st |+ (Temp (n2w h),Word v)) =
+      list_store save_regs ys st |+ (Temp (n2w h),Word v)``,
+  Induct \\ fs [list_store_def] \\ rpt strip_tac
+  \\ match_mp_tac FUPDATE_COMMUTES \\ fs [] \\ metis_tac []);
+
+val evaluate_SaveRegs = prove(
+  ``!save_regs t7 vals.
+      LIST_REL (λn v. lookup (n + 2) t7.locals = SOME (Word v)) save_regs vals /\
+      ALL_DISTINCT save_regs /\ EVERY (\n. n < max_var_name) save_regs ==>
+      evaluate (SaveRegs save_regs,t7) =
+        (NONE,t7 with store := list_store save_regs (MAP Word vals) t7.store)``,
+  Induct \\ fs [list_store_def,SaveRegs_def]
+  THEN1 (simp [Once evaluate_def,wordSemTheory.state_component_equality])
+  \\ fs [PULL_EXISTS]
+  \\ fs [evaluate_def,word_exp_def,set_store_def]
+  \\ rpt strip_tac \\ fs []
+  \\ qmatch_goalsub_abbrev_tac `evaluate (_,t99)`
+  \\ first_x_assum (qspecl_then [`t99`,`ys`] mp_tac)
+  \\ impl_tac THEN1 (unabbrev_all_tac \\ fs [])
+  \\ fs [] \\ unabbrev_all_tac \\ fs []
+  \\ fs [wordSemTheory.state_component_equality]
+  \\ rpt strip_tac
+  \\ match_mp_tac list_store_FUPDATE \\ fs []);
+
+val FLOOKUP_list_store_ignore = prove(
+  ``!save_regs vals st.
+    EVERY (λn. n < max_var_name) save_regs ==>
+    FLOOKUP (list_store save_regs vals st) TempIn1 = FLOOKUP st TempIn1 /\
+    FLOOKUP (list_store save_regs vals st) TempIn2 = FLOOKUP st TempIn2 /\
+    FLOOKUP (list_store save_regs vals st) TempOut = FLOOKUP st TempOut /\
+    !n. (!r. n <> Temp r) ==>
+        FLOOKUP (list_store save_regs vals st) n = FLOOKUP st n``,
+  Induct \\ Cases_on `vals`
+  \\ fs [list_store_def,FLOOKUP_UPDATE,
+         TempIn1_def,TempIn2_def,TempOut_def]);
+
+val copy_vars_const = prove(
+  ``!save_regs s2 s3.
+      copy_vars save_regs s1.regs s2 = SOME s3 ==>
+      s3.clock = s2.clock /\ s3.arrays = s2.arrays``,
+  Induct \\ fs [copy_vars_def] \\ rpt strip_tac \\ FULL_CASE_TAC \\ fs []
+  \\ res_tac \\ fs [reg_write_def]);
+
+val lookup_list_update_ADD_2 = prove(
+  ``!save_regs ws.
+      lookup 0 (list_update (MAP (λn. n + 2) save_regs) ws l) = lookup 0 l``,
+  Induct \\ Cases_on `ws` \\ fs [list_update_def,lookup_insert]);
+
+val copy_vars_ignore = prove(
+  ``!save_regs regs s2 s3.
+      copy_vars save_regs regs s2 = SOME s3 /\
+      ~MEM a save_regs /\ a < max_var_name /\
+      EVERY (λn. n < max_var_name) save_regs ==>
+      s3.regs ' a = s2.regs ' a``,
+  Induct \\ fs [copy_vars_def] \\ rpt strip_tac \\ FULL_CASE_TAC \\ fs []
+  \\ res_tac \\ rfs [reg_write_def,FAPPLY_FUPDATE_THM]);
+
+val copy_vars_IMP = prove(
+  ``!save_regs s2 s3.
+      copy_vars save_regs s1.regs s2 = SOME s3 ==>
+      ?vals. EVERY2 (\n v. FLOOKUP s1.regs n = SOME v) save_regs vals``,
+  Induct \\ fs [copy_vars_def] \\ rw [] \\ FULL_CASE_TAC
+  \\ fs [] \\ res_tac \\ metis_tac []);
+
+val LIST_REL_lemma = prove(
+  ``!xs ys.
+      (!x y. MEM x xs /\ MEM y ys ==> P x y ==> Q x y) ==>
+      LIST_REL P xs ys ==>
+      LIST_REL Q xs ys``,
+  Induct \\ fs [] \\ rpt strip_tac \\ rveq \\ fs []);
 
 val compile_thm = store_thm("compile_thm",
   ``!rec s1 prog s2.
@@ -813,20 +943,29 @@ val compile_thm = store_thm("compile_thm",
     \\ fs [state_rel_def] \\ fs [])
   THEN1 (* Rec *)
    (fs [compile_def] \\ rveq
-    \\ fs [compile_def,syntax_ok_def] \\ rfs []
+    \\ fs [compile_def,syntax_ok_def,syntax_ok_aux_def] \\ rfs []
     \\ simp [Once evaluate_def]
+    \\ drule copy_vars_IMP \\ strip_tac
+    \\ drule (GEN_ALL evaluate_LoadRegs)
+    \\ rpt (disch_then drule) \\ fs []
+    \\ disch_then kall_tac
     \\ simp [Once evaluate_def,find_code_def,bad_dest_args_def,add_ret_loc_def,
          get_vars_def]
-    \\ `wordSem$cut_env (LS ()) t1.locals = SOME (insert 0 ret_val LN)` by
-       (fs [wordSemTheory.cut_env_def,domain_lookup,get_var_def]
-        \\ fs [spt_eq_thm,wf_insert,wf_def,lookup_insert,
-               lookup_def,lookup_inter_alt] \\ NO_TAC) \\ fs []
+    \\ IF_CASES_TAC
+    THEN1 (fs [EXTENSION,domain_list_insert] \\ metis_tac [])
+    \\ TOP_CASE_TAC THEN1
+     (sg `F` \\ fs [] \\ pop_assum mp_tac \\ fs []
+      \\ fs [cut_env_def,domain_list_insert,SUBSET_DEF,get_var_def]
+      \\ fs [domain_list_update]
+      \\ fs [domain_lookup] \\ metis_tac [])
     \\ `t1.clock <> 0` by fs [state_rel_def] \\ fs []
     \\ qmatch_goalsub_abbrev_tac `evaluate (_,t6)`
     \\ first_x_assum drule \\ fs []
     \\ disch_then (qspecl_then [`cs2`,`t6`,`Loc n l`] mp_tac)
     \\ impl_tac THEN1
-     (`t6.code = t1.code` by (fs [Abbr `t6`] \\ EVAL_TAC \\ fs []) \\ fs []
+     (`t6.code = t1.code` by
+       (unabbrev_all_tac \\ fs [call_env_def,push_env_def]
+        \\ pairarg_tac \\ fs [] \\ EVAL_TAC) \\ fs []
       \\ conj_tac THEN1
        (match_mp_tac state_rel_delete_vars
         \\ fs [state_rel_def,dec_clock_def,wordSemTheory.dec_clock_def,Abbr`t6`,
@@ -834,18 +973,89 @@ val compile_thm = store_thm("compile_thm",
         \\ pairarg_tac \\ fs [])
       \\ fs [PULL_EXISTS]
       \\ asm_exists_tac \\ fs []
-      \\ unabbrev_all_tac \\ EVAL_TAC)
+      \\ unabbrev_all_tac \\ fs [call_env_def,push_env_def]
+      \\ pairarg_tac \\ fs [] \\ EVAL_TAC)
     \\ strip_tac \\ fs []
     \\ simp [Once evaluate_def]
     \\ fs [pop_env_def,call_env_def,push_env_def]
     \\ fs [env_to_list_insert_0_LN,EVAL ``domain (fromAList [(0,ret_val)])``]
     \\ qunabbrev_tac `t6` \\ fs []
     \\ fs [set_var_def,fromAList_def,wordSemTheory.dec_clock_def]
-    \\ simp [Once evaluate_def]
+    \\ Cases_on `env_to_list x t1.permute` \\ fs []
+    \\ reverse IF_CASES_TAC THEN1
+     (sg `F` \\ fs [] \\ pop_assum mp_tac
+      \\ imp_res_tac env_to_list_lookup_equiv
+      \\ simp [EXTENSION,domain_lookup,lookup_fromAList])
+    \\ qmatch_goalsub_abbrev_tac `evaluate (_,t7)`
+    \\ `EVERY2 (λn v. lookup (n+2) t7.locals = SOME (Word v)) save_regs vals` by
+     (fs [cut_env_def] \\ rveq \\ unabbrev_all_tac
+      \\ fs [lookup_insert,lookup_fromAList]
+      \\ imp_res_tac env_to_list_lookup_equiv
+      \\ fs [lookup_inter_alt,domain_list_insert]
+      \\ imp_res_tac EVERY2_LENGTH
+      \\ pop_assum mp_tac
+      \\ qpat_x_assum `ALL_DISTINCT save_regs` mp_tac
+      \\ rpt (pop_assum kall_tac)
+      \\ qspec_tac (`vals`,`vals`)
+      \\ qspec_tac (`save_regs`,`save_regs`)
+      \\ Induct \\ fs []
+      \\ Cases_on `vals` \\ fs [list_update_def,lookup_insert]
+      \\ rpt strip_tac
+      \\ res_tac \\ pop_assum mp_tac
+      \\ match_mp_tac LIST_REL_lemma \\ fs [] \\ metis_tac [])
+    \\ drule (GEN_ALL evaluate_SaveRegs) \\ fs []
+    \\ disch_then kall_tac \\ qunabbrev_tac `t7`
     \\ Q.MATCH_GOALSUB_ABBREV_TAC `(p9,t8)`
     \\ qexists_tac `t8` \\ fs []
     \\ unabbrev_all_tac \\ fs [get_var_def,lookup_insert]
-    \\ fs [state_rel_def] \\ fs [])
+    \\ imp_res_tac env_to_list_lookup_equiv
+    \\ fs [lookup_fromAList,get_var_def,state_rel_def]
+    \\ imp_res_tac copy_vars_const
+    \\ `lookup 0 x = SOME ret_val` by
+      (fs [cut_env_def] \\ rveq
+       \\ fs [lookup_inter_alt,domain_list_insert,lookup_list_update_ADD_2])
+    \\ fs [FLOOKUP_list_store_ignore]
+    \\ qpat_x_assum `LIST_REL (λn v. FLOOKUP s1.regs n = SOME v) save_regs vals`
+          mp_tac
+    \\ qpat_x_assum `!x y. _` kall_tac
+    \\ qpat_x_assum `!x y. _` mp_tac
+    \\ qpat_x_assum `EVERY (λn. n < _) save_regs` mp_tac
+    \\ qpat_x_assum `ALL_DISTINCT save_regs` mp_tac
+    \\ qpat_x_assum `copy_vars save_regs s1.regs s2 = SOME s3` mp_tac
+    \\ rpt (pop_assum kall_tac)
+    \\ qspec_tac (`t2.store`,`st`)
+    \\ qspec_tac (`s1.regs`,`regs`)
+    \\ qspec_tac (`vals`,`vals`)
+    \\ qspec_tac (`s2`,`s2`)
+    \\ qspec_tac (`s3`,`s3`)
+    \\ qspec_tac (`save_regs`,`save_regs`)
+    \\ Induct \\ fs [copy_vars_def,list_store_def,PULL_EXISTS]
+    \\ simp_tac std_ss [PULL_FORALL,AND_IMP_INTRO]
+    \\ rpt gen_tac \\ strip_tac
+    \\ fs [GSYM PULL_FORALL]
+    \\ Cases_on `FLOOKUP regs h` \\ fs [] \\ rveq \\ fs []
+    \\ Cases_on `a = h` THEN1
+     (rveq \\ fs [FLOOKUP_DEF,FAPPLY_FUPDATE_THM] \\ rveq
+      \\ imp_res_tac copy_vars_ignore \\ fs [] \\ EVAL_TAC)
+    \\ first_x_assum drule
+    \\ disch_then (qspecl_then [`ys`,`st |+ (Temp (n2w h),Word v)`] mp_tac)
+    \\ fs []
+    \\ impl_tac THEN1
+     (fs [reg_write_def,FLOOKUP_DEF,FAPPLY_FUPDATE_THM] \\ ntac 2 strip_tac
+      \\ rveq \\ fs [] \\ res_tac \\ fs [] \\ rw [])
+    \\ disch_then drule \\ fs []
+    \\ qsuff_tac
+       `(list_store save_regs (MAP Word ys) (st |+ (Temp (n2w h),Word v))) =
+        (list_store save_regs (MAP Word ys) st) |+ (Temp (n2w h),Word v)` \\ fs []
+    \\ qpat_x_assum `EVERY _ _` mp_tac
+    \\ qpat_x_assum `_ < _:num` mp_tac
+    \\ qpat_x_assum `~(MEM _ _)` mp_tac
+    \\ qspec_tac (`MAP Word ys`,`zs`)
+    \\ qspec_tac (`st`,`st`)
+    \\ rpt (pop_assum kall_tac)
+    \\ Induct_on `save_regs` \\ fs [list_store_def]
+    \\ rpt strip_tac \\ fs []
+    \\ match_mp_tac FUPDATE_COMMUTES \\ fs [])
   THEN1 (* LoopBody ret *)
    (fs [syntax_ok_def,compile_def]
     \\ `syntax_ok prog /\ !r. prog <> LoopBody r` by
@@ -975,8 +1185,7 @@ val Corr_Seq = prove(
     Corr p1 s (INR s1) q1 ==>
     Corr (Seq p1 p2) s s2 (q1 /\ q2)``,
   fs [Corr_def,eval_cases] \\ rw [] \\ fs []
-  \\ asm_exists_tac \\ fs []
-  \\ imp_res_tac Eval_INR_loop \\ fs []);
+  \\ asm_exists_tac \\ fs []);
 
 val Corr_Seq_alt = prove(
   ``(b ==> Corr p2 s1 s2 q2) ==>
@@ -1471,11 +1680,11 @@ local val s = HolKernel.syntax_fns1 "word_bignum" in
 end
 local val s = HolKernel.syntax_fns2 "word_bignum" in
   val (Assign_tm,mk_Assign,dest_Assign,is_Assign) = s "Assign"
-  val (Loop_tm,mk_Loop,dest_Loop,is_Loop) = s "Loop"
   val (Seq_tm,mk_Seq,dest_Seq,is_Seq) = s "Seq"
   val (Store_tm,mk_Store,dest_Store,is_Store) = s "Store"
 end
 local val s = HolKernel.syntax_fns3 "word_bignum" in
+  val (Loop_tm,mk_Loop,dest_Loop,is_Loop) = s "Loop"
   val (Load_tm,mk_Load,dest_Load,is_Load) = s "Load"
 end
 
